Initial stuff for symbolic type reconstruction

theories/stlc/Symbolic.v
@@ -160,3 +160,50 @@ Section RunTI.
     ground ctx.nil env.nil (infer_ng e).
 
 End RunTI.
+
+Section TypeReconstruction.
+
+  Definition Prod A B : Ctx nat -> Type := fun w => prod (A w) (B w).
+  Definition Expr : Ctx nat -> Type := fun _ => expr.
+
+  Instance Persistent_Prod : forall A B, Persistent A -> Persistent B -> Persistent (Prod A B).
+  Proof. firstorder. Qed.
+
+  Definition ret {w} := Ret_Free (Prod Ty Expr) w.
+  Definition fail {w} := Fail_Free (Prod Ty Expr) w.
+
+Fixpoint generate' (e : expr) {Σ : Ctx nat} (Γ : Env Σ) : FreeM (Prod Ty Expr) Σ.
+refine (
+  match e with
+  | v_true  => ret (Ty_bool Σ, v_true)
+  | v_false => ret (Ty_bool Σ, v_false)
+  | e_if cnd coq alt =>
+      [ ω1 ] r_cnd <- generate' cnd _ Γ ;;
+      [ ω2 ] _     <- assert (fst r_cnd) (Ty_bool _) ;;
+      [ ω3 ] r_coq <- generate' coq _ <{ Γ ~ ω1 .> ω2 }> ;;
+      [ ω4 ] r_alt <- generate' alt _ <{ Γ ~ ω1 .> ω2 .> ω3 }> ;;
+      [ ω5 ] _     <- assert <{ (fst r_coq) ~ ω4 }>  <{ (fst r_alt) ~ (refl _) }> ;;
+         ret (<{ fst r_coq ~ ω4 .> ω5 }>, e_if (snd r_cnd) (snd r_coq) (snd r_alt))
+  | e_var var =>
+      match (value var Γ) with
+      | Some t_var => ret (t_var, e_var var)
+      | None => fail
+      end
+  | e_app f a =>
+      [ ω1 ] t_co <- exists_Ty Σ ;;
+      [ ω2 ] t_do <- generate' a _ <{ Γ ~ ω1 }> ;;
+      [ ω3 ] t_fn <- generate' f _ <{ Γ ~ ω1 .> ω2 }> ;;
+      [ ω4 ] _    <- assert (fst t_fn) <{ (Ty_func _ (fst t_do) <{ t_co ~ ω2 }> ) ~ ω3 }> ;;
+          ret (<{ t_co ~ ω2 .> (ω3 .> ω4) }>, e_app (snd t_fn) (snd t_do))
+  | e_abst var t_var e =>
+      let t_var' := (lift t_var Σ) in (* t_var lives in ty, not in (Ty w) *)
+      [ ω1 ] t_e <- generate' e _ ((var, t_var') :: Γ) ;;
+        ret (Ty_func _ <{ t_var' ~ ω1 }> (fst t_e), e_abst var t_var (snd t_e))
+  | e_absu var e =>
+      [ ω1 ] t_var <- exists_Ty Σ ;;
+      [ ω2 ] t_e <- generate' e _ ((var, t_var) :: <{ Γ ~ ω1 }>) ;;
+        ret (Ty_func _ <{ t_var ~ ω2 }> (fst t_e), e_abst var _ (snd t_e))
+  end).
+Proof. Admitted.
+
+End TypeReconstruction.
